We derive the convenience yield coefficients for both the Leontief and Cobb-Douglas matching functions, showing that despite different dynamics, they yield identical functional forms.

\subsection{Verification for the Leontief Case ($\theta_0 > 1$)}

\textbf{Step 1: Specialize market dynamics.}
With the Leontief matching function, from Table \ref{tab:closedforms} we have:
\[
\theta_{\tau} = 1 + (\theta_0 - 1)e^{\bar{\lambda}\tau},\quad \psi^+_{\tau} = \bar{\lambda}, \quad \psi^-_{\tau}= \frac{\bar{\lambda}}{\theta_{\tau}} = \frac{\bar{\lambda}}{1 + (\theta_0 - 1)e^{\bar{\lambda}\tau}}
\]
The terminal tightness is $\bar{\theta} = \theta_1 = 1 + (\theta_0 - 1)e^{\bar{\lambda}}$. Thus, we compute the following integrals:
\begin{align*}
\int_t^1 \psi_\tau^+ \, d\tau = \int_t^1 \bar{\lambda} \, d\tau &= \bar{\lambda}(1-t),
\end{align*}
and
\begin{align*}
 \int_t^1 \psi_\tau^- \, d\tau = \int_t^1 \frac{\bar{\lambda}}{1 + (\theta_0 - 1)e^{\bar{\lambda}\tau}} \, d\tau
&= \Big[\bar{\lambda}\tau - \ln\big(1 + (\theta_0 - 1)e^{\bar{\lambda}\tau}\big)\Big]_t^1\\
&= \bar{\lambda}(1-t) - \ln\left(\frac{1 + (\theta_0 - 1)e^{\bar{\lambda}}}{1 + (\theta_0 - 1)e^{\bar{\lambda}t}}\right).
\end{align*}

The convenience yield coefficients (outside options) take the following forms::
\begin{equation}
\chi_\tau^+ = (1-\eta)(r^w - r^m)\mathbb{P}_\tau^+ \quad \text{and} \quad \chi_\tau^- = (r^w - r^m)(1 - \eta\mathbb{P}_\tau^-),
\end{equation}
where
\begin{align*}
\mathbb{P}_t^+ &= \int_t^1 \psi_\tau^+ e^{-[\eta\Psi_\tau^- + (1-\eta)\Psi_\tau^+]} \, d\tau\\
&= \int_t^1 \bar{\lambda} e^{-\bar{\lambda}(1-\tau) + \eta\ln\left(\frac{1 + (\theta_0 - 1)e^{\bar{\lambda}}}{1 + (\theta_0 - 1)e^{\bar{\lambda}\tau}}\right)} \, d\tau\\
&= \int_t^1 \left(\frac{1 + (\theta_0 - 1)e^{\bar{\lambda}}}{1 + (\theta_0 - 1)e^{\bar{\lambda}\tau}}\right)^{\eta} \bar{\lambda} e^{-\bar{\lambda}(1-\tau)} \, d\tau\\
&= \left[\frac{1 + (\theta_0 - 1)e^{\bar{\lambda}\tau}}{(1-\eta)(\theta_0 - 1)e^{\bar{\lambda}}} \left(\frac{1 + (\theta_0 - 1)e^{\bar{\lambda}}}{1 + (\theta_0 - 1)e^{\bar{\lambda}\tau}}\right)^{\eta}\right]_t^1\\
&= \frac{1 + (\theta_0 - 1)e^{\bar{\lambda}}}{(1-\eta)(\theta_0 - 1)e^{\bar{\lambda}}} - \frac{1 + (\theta_0 - 1)e^{\bar{\lambda}t}}{(1-\eta)(\theta_0 - 1)e^{\bar{\lambda}}} \left(\frac{1 + (\theta_0 - 1)e^{\bar{\lambda}}}{1 + (\theta_0 - 1)e^{\bar{\lambda}t}}\right)^{\eta}\\
&= \frac{\theta_1\left(1 - \left(\frac{\theta_t}{\theta_1}\right)^{1-\eta}\right)}{(1-\eta)(\theta_1 - 1)} = \frac{1}{1-\eta} \cdot \frac{\theta_1 - \theta_t^{1-\eta}\theta_1^{\eta}}{\theta_1 - 1}\\
&= \frac{1}{1-\eta} \left(\frac{\bar{\theta}}{\theta}\right)^{\eta} \left(\frac{\theta^{\eta}\bar{\theta}^{1-\eta} - \theta}{\bar{\theta} - 1}\right).
\end{align*}
and where
\begin{align*}
\mathbb{P}_t^- &= \int_t^1 \psi_\tau^- e^{-[\eta\Psi_\tau^- + (1-\eta)\Psi_\tau^+]} \, d\tau\\
&= \int_t^1 \left(\frac{\bar{\lambda}}{1 + (\theta_0 - 1)e^{\bar{\lambda}\tau}}\right) e^{-\bar{\lambda}(1-\tau) + \eta\ln\left(\frac{1 + (\theta_0 - 1)e^{\bar{\lambda}}}{1 + (\theta_0 - 1)e^{\bar{\lambda}\tau}}\right)} \, d\tau\\
&= \int_t^1 \left(\frac{1 + (\theta_0 - 1)e^{\bar{\lambda}}}{1 + (\theta_0 - 1)e^{\bar{\lambda}\tau}}\right)^{\eta} \left(\frac{\bar{\lambda}e^{-\bar{\lambda}(1-\tau)}}{1 + (\theta_0 - 1)e^{\bar{\lambda}\tau}}\right) \, d\tau\\
&= \left[\left(\frac{-1}{\eta(\theta_0 - 1)e^{\bar{\lambda}}}\right) \left(\frac{1 + (\theta_0 - 1)e^{\bar{\lambda}}}{1 + (\theta_0 - 1)e^{\bar{\lambda}\tau}}\right)^{\eta}\right]_t^1\\
&= \frac{1}{\eta(\theta_0 - 1)e^{\bar{\lambda}}} \left(\frac{1 + (\theta_0 - 1)e^{\bar{\lambda}}}{1 + (\theta_0 - 1)e^{\bar{\lambda}t}}\right)^{\eta} - \frac{1}{\eta(\theta_0 - 1)e^{\bar{\lambda}}}\\
&= \frac{\left(\frac{\theta_1}{\theta_t}\right)^{\eta} - 1}{\eta(\theta_1 - 1)}.
\end{align*}
Thus, we obtain the following formulas:
\begin{equation*}
\chi_\tau^+ = (r^w - r^m)\left(\frac{\theta_1}{\theta_\tau}\right)^{\eta} \left(\frac{\theta_\tau^{\eta}\theta_1^{1-\eta} - \theta_\tau}{\theta_1 - 1}\right)\quad
\chi_\tau^- = (r^w - r^m)\left(\frac{\theta_1}{\theta_\tau}\right)^{\eta} \left(\frac{\theta_\tau^{\eta}\theta_1^{1-\eta} - 1}{\theta_1 - 1}\right).
\end{equation*}
From here, substitute for $\tau = 0$ and obtain $\{\chi_0^+, \chi_0^-\}$.

\subsection{Leontief Case ($\theta_0 < 1$) via Symmetry}

For $\theta_0 < 1$, we can apply the symmetry property from Proposition \ref{prop:symmetry} rather than repeat the calculations.
\[
\chi^{+}(\theta_0, \eta) = (r^{w}-r^{m}) - \chi^{-}(\theta_0^{-1}, 1-\eta).
\]
Since $\theta_0^{-1} > 1$, we can use our formula:
\[
\chi^{-}(\theta_0^{-1}, 1-\eta) = (r^{w}-r^{m})\frac{\bar{\theta}^{-1} - (\bar{\theta}^{-1})^{1-\eta}(\theta_0^{-1})^{-(1-\eta)}}{\bar{\theta}^{-1}-1}=(r^{w}-r^{m})\frac{1 - \bar{\theta}^{\eta}\theta_0^{(1-\eta)}}{1-\bar{\theta}}.
\]
Thus, we have that:
\[
\chi^{+}(\theta_0, \eta) = (r^{w}-r^{m})\left(1-\frac{1 - \bar{\theta}^{\eta}\theta_0^{(1-\eta)}}{1-\bar{\theta}}\right)=(r^{w}-r^{m})\left(\frac{\bar{\theta} - \bar{\theta}^{\eta}\theta_0^{(1-\eta)}}{\bar{\theta}-1}\right).
\]
Thus, the same formula is valid for $\chi^{+}(\theta_0, \eta)$ regardless of whether $\theta_0>1$ or $\theta_0<1.$ Since the formula for $\chi^{+}$ holds when $\theta_0<1$, the formula for $\chi^{-}$ must also hold in both cases. 

\subsection{Cobb-Douglas Case}
{\color{red}
TBA
}

\textbf{Step 1: Specialize market dynamics.} With the Cobb-Douglas matching function:
\[
\theta_{\tau} = \left(\frac{(1+\sqrt{\theta_0})e^{-\bar{\lambda}\tau} - (1-\sqrt{\theta_0})}{(1+\sqrt{\theta_0})e^{-\bar{\lambda}\tau} + (1-\sqrt{\theta_0})}\right)^2,\quad
\psi^+_{\tau} = \bar{\lambda}\sqrt{\theta_{\tau}},\quad
\psi^-_{\tau} = \frac{\bar{\lambda}}{\sqrt{\theta_{\tau}}}.
\]
Define $u = e^{-\bar{\lambda}\tau}$. Then:
\[
\theta_\tau = \left(\frac{\alpha u - 1}{\alpha u + 1}\right)^2.
\]


\textbf{Step 2: Computing the surplus}
The surplus at time $\tau$ is:
\[
\Sigma_\tau = (r^w - r^m)\exp\left(-\int_\tau^T [\eta\psi_s^- + (1-\eta)\psi_s^+] ds\right)
\]

From previous calculations:
\begin{align}
\int_\tau^T \psi_s^- ds &= \ln\left(\frac{\alpha - e^{\bar{\lambda}T}}{\alpha + e^{\bar{\lambda}T}}\right) - \ln\left(\frac{\alpha - e^{\bar{\lambda}\tau}}{\alpha + e^{\bar{\lambda}\tau}}\right)\\
\int_\tau^T \psi_s^+ ds &= \ln\left(\frac{\alpha + e^{\bar{\lambda}\tau}}{\alpha - e^{\bar{\lambda}\tau}}\right) - \ln\left(\frac{\alpha + e^{\bar{\lambda}T}}{\alpha - e^{\bar{\lambda}T}}\right)
\end{align}

For stopping time $T$ (when exhaustion occurs): $\alpha e^{-\bar{\lambda}T} = 1 \implies T = \frac{1}{\bar{\lambda}}\ln(\alpha)$

\textbf{Step 4: Computing $\mathbb{P}_t^+$}
Starting with:
\[
\mathbb{P}_t^+ = \int_t^T \psi_\tau^+ e^{-[\eta\Psi_\tau^- + (1-\eta)\Psi_\tau^+]} d\tau
\]

Substituting the exponent terms:
\begin{align}
\mathbb{P}_t^+ &= \int_t^T \bar{\lambda}\sqrt{\theta_\tau} \exp\left[-\eta\ln\left(\frac{\alpha - e^{\bar{\lambda}T}}{\alpha + e^{\bar{\lambda}T}} \cdot \frac{\alpha + e^{\bar{\lambda}\tau}}{\alpha - e^{\bar{\lambda}\tau}}\right)\right.\\
&\qquad\qquad\qquad\quad \left.-(1-\eta)\ln\left(\frac{\alpha + e^{\bar{\lambda}\tau}}{\alpha - e^{\bar{\lambda}\tau}} \cdot \frac{\alpha - e^{\bar{\lambda}T}}{\alpha + e^{\bar{\lambda}T}}\right)\right] d\tau
\end{align}

Simplifying the exponential:
\[
\mathbb{P}_t^+ = \int_t^T \bar{\lambda}\left(\frac{\alpha e^{-\bar{\lambda}\tau} - 1}{\alpha e^{-\bar{\lambda}\tau} + 1}\right) \left(\frac{\alpha - e^{\bar{\lambda}T}}{\alpha + e^{\bar{\lambda}T}}\right)^{-\eta} \left(\frac{\alpha + e^{\bar{\lambda}\tau}}{\alpha - e^{\bar{\lambda}\tau}}\right)^{-\eta} \left(\frac{\alpha + e^{\bar{\lambda}\tau}}{\alpha - e^{\bar{\lambda}\tau}}\right)^{-(1-\eta)} d\tau
\]

This simplifies to:
\[
\mathbb{P}_t^+ = \int_t^T \bar{\lambda}\left(\frac{\alpha e^{-\bar{\lambda}\tau} - 1}{\alpha e^{-\bar{\lambda}\tau} + 1}\right) \left(\frac{\alpha - e^{\bar{\lambda}T}}{\alpha + e^{\bar{\lambda}T}}\right)^{-\eta} \left(\frac{\alpha - e^{\bar{\lambda}\tau}}{\alpha + e^{\bar{\lambda}\tau}}\right) d\tau
\]

Using substitution $u = e^{-\bar{\lambda}\tau}$, $du = -\bar{\lambda}e^{-\bar{\lambda}\tau}d\tau = -\bar{\lambda}u \, d\tau$:
\[
\mathbb{P}_t^+ = \int_{e^{-\bar{\lambda}t}}^{1/\alpha} \left(\frac{\alpha u - 1}{\alpha u + 1}\right) \left(\frac{\alpha - 1}{\alpha + 1}\right)^{-\eta} \left(\frac{\alpha - 1/u}{\alpha + 1/u}\right) \left(-\frac{du}{u}\right)
\]

After integration:
\[
\mathbb{P}_t^+ = \frac{1}{2\alpha(1-\eta)} \left[\frac{\alpha e^{-\bar{\lambda}t} + 1}{\alpha e^{-\bar{\lambda}t} - 1} \left(\frac{\alpha - e^{\bar{\lambda}t}}{\alpha + e^{\bar{\lambda}t}}\right)^{\eta} - \frac{2\alpha}{1-\eta}\right]
\]

\textbf{Step 5: Computing $\mathbb{P}_t^-$}
Similarly:
\[
\mathbb{P}_t^- = \int_t^T \psi_\tau^- e^{-[\eta\Psi_\tau^- + (1-\eta)\Psi_\tau^+]} d\tau
\]

With full exponent terms:
\[
\mathbb{P}_t^- = \int_t^T \frac{\bar{\lambda}}{\sqrt{\theta_\tau}} \left(\frac{\alpha - e^{\bar{\lambda}T}}{\alpha + e^{\bar{\lambda}T}}\right)^{-\eta} \left(\frac{\alpha + e^{\bar{\lambda}\tau}}{\alpha - e^{\bar{\lambda}\tau}}\right)^{-\eta} \left(\frac{\alpha + e^{\bar{\lambda}\tau}}{\alpha - e^{\bar{\lambda}\tau}}\right)^{-(1-\eta)} d\tau
\]

After simplification and integration:
\[
\mathbb{P}_t^- = \frac{1}{\eta}\left[\left(\frac{\alpha - e^{\bar{\lambda}t}}{\alpha + e^{\bar{\lambda}t}}\right)^{\eta} - \left(\frac{\alpha - 1}{\alpha + 1}\right)^{\eta}\right]
\]

\textbf{Step 6: Final expressions for $\chi^+$ and $\chi^-$}
Setting $t = 0$ and using the relationships:
\[
\chi^+ = (r^w - r^m)\frac{\bar{\theta} - \bar{\theta}^{\eta}\theta_0^{1-\eta}}{\bar{\theta} - 1}, \quad
\chi^- = (r^w - r^m)\frac{\bar{\theta} - \bar{\theta}^{\eta}\theta_0^{-\eta}}{\bar{\theta} - 1}
\]

